Min max functions support added. Dafny verification improved to support more complex reducers.

bin/benchmarks/Aggregation/Delta.java
@@ -8,8 +8,8 @@ public class Delta {
 	}
 	
 	public static int deltaList(List<Integer> data) {
-		int max = 0;
-		int min = 0;
+		int max = Integer.MIN_VALUE;
+		int min = Integer.MAX_VALUE;
 		for(int i=0; i<data.size(); i++) {
 			int var = data.get(i);
 			max = Math.max(var,max);
