bin/benchmarks/Aggregation/MaxAbs.java
@@ -8,11 +8,11 @@ public class MaxAbs {
 	}
 	
 	public static int maxAbsList(List<Integer> data) {
-		int maxAbs = 0;
+		int maxAbs = Integer.MIN_VALUE;
 		for(int i=0; i<data.size(); i++) {
 			int var = data.get(i);
 			maxAbs = Math.max(Math.abs(var),maxAbs);
 		}
 		return maxAbs;
 	}
-}n
+}
