bin/templates/dafny_skeleton.dfy
@@ -24,6 +24,7 @@ function mapper (<mapper-args-decl>) : <domap-emit-type>
 }
 
 /***************************** DO REDUCE ************************************/
+<reduce-functions>
 
 function doreduce(input: <domap-emit-type>, key: <doreduce-key-type><reducer-args-decl>) : <output-type>
     ensures (|input| > 0 && input[0].0 == key) ==> 
